adapt: include rho in value relation

theories/CodegenWASM/LambdaANF_to_WASM_correct.v
@@ -493,8 +493,13 @@ Let store_record := store_record host_function.
 
 (* VALUE RELATION *)
 (* immediate is pointer to linear memory or function id *)
-Inductive repr_val_LambdaANF_Codegen:  LambdaANF.cps.val -> store_record -> frame -> wasm_value -> Prop :=
-| Rconstr_v : forall v t vs (sr : store_record) fr gmp m (addr : nat),
+Inductive repr_val_LambdaANF_Codegen: LambdaANF.eval.env -> (* rho *)
+                                       LambdaANF.cps.val -> (* val *)
+                                        store_record ->     (* sr *)
+                                         frame ->           (* fr *)
+                                          wasm_value ->     (* wal *)
+                                           Prop :=
+| Rconstr_v : forall rho v t vs (sr : store_record) fr gmp m (addr : nat),
     (* only depends on memory before v_gmp (simple memory model: gmp is increased whenever new mem is needed) *)
     sglob_val (host_function:=host_function) sr (f_inst fr) global_mem_ptr = Some (VAL_int32 (nat_to_i32 gmp)) ->
     (-1 < Z.of_nat gmp < Wasm_int.Int32.modulus)%Z ->
@@ -506,9 +511,10 @@ Inductive repr_val_LambdaANF_Codegen:  LambdaANF.cps.val -> store_record -> fram
     v = tag_to_i32 t ->
     load_i32 m (N.of_nat addr) = Some (VAL_int32 v) ->
     (* arguments are set properly *)
-    repr_val_constr_args_LambdaANF_Codegen vs sr fr (4 + addr) ->
-    repr_val_LambdaANF_Codegen (LambdaANF.cps.Vconstr t vs) sr fr (Val_ptr addr)
-| Rfunction_v : forall env fds f sr fr tag vs e e' idx inst ftype args body,
+    repr_val_constr_args_LambdaANF_Codegen rho vs sr fr (4 + addr) ->
+    repr_val_LambdaANF_Codegen rho (LambdaANF.cps.Vconstr t vs) sr fr (Val_ptr addr)
+| Rfunction_v : forall x rho rho' env fds f sr fr tag vs e e' idx inst ftype args body,
+      M.get x rho = Some (Vfun rho' fds f) ->
       find_def f fds = Some (tag, vs, e) ->
 
       (* find runtime representation of function *)
@@ -518,13 +524,13 @@ Inductive repr_val_LambdaANF_Codegen:  LambdaANF.cps.val -> store_record -> fram
       repr_expr_LambdaANF_Codegen e e'
         (lenv:=create_local_variable_mapping (collect_local_variables e)) ->
       (* env: why empty? *)
-      repr_val_LambdaANF_Codegen (LambdaANF.cps.Vfun env fds f) sr fr (Val_funidx idx)
+      repr_val_LambdaANF_Codegen rho (LambdaANF.cps.Vfun env fds f) sr fr (Val_funidx idx)
 
-with repr_val_constr_args_LambdaANF_Codegen : (list LambdaANF.cps.val) -> store_record -> frame -> immediate -> Prop :=
-     | Rnil_l : forall sr fr addr,
-        repr_val_constr_args_LambdaANF_Codegen nil sr fr (addr : nat)
+with repr_val_constr_args_LambdaANF_Codegen : LambdaANF.eval.env -> list LambdaANF.cps.val -> store_record -> frame -> immediate -> Prop :=
+     | Rnil_l : forall rho sr fr addr,
+        repr_val_constr_args_LambdaANF_Codegen rho nil sr fr (addr : nat)
 
-     | Rcons_l: forall v wal vs sr fr m addr gmp,
+     | Rcons_l: forall rho v wal vs sr fr m addr gmp,
         (* store_record contains memory *)
         List.nth_error sr.(s_mems) 0 = Some m ->
 
@@ -534,11 +540,11 @@ with repr_val_constr_args_LambdaANF_Codegen : (list LambdaANF.cps.val) -> store_
 
         (* constr arg is ptr related to value v *)
         load_i32 m (N.of_nat addr) = Some (VAL_int32 (wasm_value_to_i32 wal)) ->
-        repr_val_LambdaANF_Codegen v sr fr wal ->
+        repr_val_LambdaANF_Codegen rho v sr fr wal ->
 
         (* following constr args are also related *)
-        repr_val_constr_args_LambdaANF_Codegen vs sr fr (4 + addr) ->
-        repr_val_constr_args_LambdaANF_Codegen (v::vs) sr fr addr.
+        repr_val_constr_args_LambdaANF_Codegen rho vs sr fr (4 + addr) ->
+        repr_val_constr_args_LambdaANF_Codegen rho (v::vs) sr fr addr.
 
 Scheme repr_val_LambdaANF_Codegen_mut := Induction for repr_val_LambdaANF_Codegen Sort Prop
   with repr_val_constr_args_LambdaANF_Codegen_mut := Induction for repr_val_constr_args_LambdaANF_Codegen Sort Prop.
@@ -754,7 +760,7 @@ Definition rel_mem_LambdaANF_Codegen {lenv} (e : exp) (rho : LambdaANF.eval.env)
             subval_or_eq (Vfun rho' fds f) v ->
             (* i is index of function f *)
             exists i, translate_function_var nenv fenv f errMsg = Ret i /\
-            repr_val_LambdaANF_Codegen (Vfun rho' fds f) sr fr (Val_funidx i) /\
+            repr_val_LambdaANF_Codegen rho (Vfun rho' fds f) sr fr (Val_funidx i) /\
             closed_val (Vfun rho' fds f))
         /\
         (* free variables are related to local var containing a memory pointer or a function index *)
@@ -763,7 +769,7 @@ Definition rel_mem_LambdaANF_Codegen {lenv} (e : exp) (rho : LambdaANF.eval.env)
             (exists v6 val,
                M.get x rho = Some v6 /\
                stored_in_locals (lenv:=lenv) x val fr /\
-               repr_val_LambdaANF_Codegen v6 sr fr val)).
+               repr_val_LambdaANF_Codegen rho v6 sr fr val)).
 
 End RELATION.
 
@@ -1196,14 +1202,14 @@ Definition finfo_env_correct :=
 
 *)
 
-Definition result_val_LambdaANF_Codegen
- (val : LambdaANF.cps.val) (sr : store_record) (fr : frame) : Prop :=
+Definition result_val_LambdaANF_Codegen (rho : LambdaANF.eval.env) (val : LambdaANF.cps.val)
+                                        (sr : store_record) (fr : frame) : Prop :=
 
    (exists res_i32 wasmval,
       (* global var *result_var* contains correct return value *)
       sglob_val sr (f_inst fr) result_var = Some (VAL_int32 res_i32) /\
       wasm_value_to_i32 wasmval = res_i32 /\
-      repr_val_LambdaANF_Codegen fenv nenv  _ val sr fr wasmval)
+      repr_val_LambdaANF_Codegen fenv nenv  _ rho val sr fr wasmval)
     \/ (sglob_val sr (f_inst fr) result_out_of_mem = Some (nat_to_value 1)).
 
 Import ssrfun ssrbool eqtype seq.
@@ -1231,25 +1237,25 @@ Proof.
   rewrite (Wasm_int.Int32.Z_lt_irrelevant high high'). reflexivity.
 Qed.
 
-Lemma val_relation_depends_on_finst : forall v sr fr fr' value,
+Lemma val_relation_depends_on_finst : forall rho v sr fr fr' value,
     f_inst fr = f_inst fr' ->
-    repr_val_LambdaANF_Codegen fenv nenv host_function v sr fr value ->
-    repr_val_LambdaANF_Codegen fenv nenv host_function v sr fr' value.
+    repr_val_LambdaANF_Codegen fenv nenv host_function rho v sr fr value ->
+    repr_val_LambdaANF_Codegen fenv nenv host_function rho v sr fr' value.
 Proof.
   intros. inv H0.
   (* constructor value *)
   { have indPrinciple := repr_val_constr_args_LambdaANF_Codegen_mut fenv nenv host_function
-    (fun (v : cps.val) (s : datatypes.store_record host_function) (f : frame) (w : wasm_value)
-                       (H: repr_val_LambdaANF_Codegen fenv nenv host_function v s f w) =>
+    (fun (rho : LambdaANF.eval.env) (v : cps.val) (s : datatypes.store_record host_function) (f : frame) (w : wasm_value)
+                       (H: repr_val_LambdaANF_Codegen fenv nenv host_function rho v s f w) =>
          (forall f',
                 f_inst f = f_inst f' ->
-                repr_val_LambdaANF_Codegen fenv nenv host_function v s f' w)
+                repr_val_LambdaANF_Codegen fenv nenv host_function rho v s f' w)
     )
-    (fun (l : seq cps.val) (s : datatypes.store_record host_function) (f : frame) (i : immediate)
-                       (H: repr_val_constr_args_LambdaANF_Codegen fenv nenv host_function l s f i) =>
+    (fun (rho : LambdaANF.eval.env) (l : seq cps.val) (s : datatypes.store_record host_function) (f : frame) (i : immediate)
+                       (H: repr_val_constr_args_LambdaANF_Codegen fenv nenv host_function rho l s f i) =>
          (forall f',
                 f_inst f = f_inst f' ->
-                repr_val_constr_args_LambdaANF_Codegen fenv nenv host_function l s f' i)
+                repr_val_constr_args_LambdaANF_Codegen fenv nenv host_function rho l s f' i)
     ). eapply indPrinciple in H7; intros; clear indPrinciple; try eassumption.
     { econstructor; eauto. congruence. }
     { econstructor; eauto. congruence. }
@@ -1261,7 +1267,39 @@ Proof.
   { econstructor; eauto. }
 Qed.
 
-Lemma val_relation_depends_on_mem_smaller_than_gmp_and_funcs : forall v sr sr' m m' fr fr' gmp gmp' value,
+Lemma val_relation_rho_depends_on_bound_vars : forall rho x v val sr fr wal,
+  rho ! x = None ->
+  repr_val_LambdaANF_Codegen fenv nenv host_function rho val sr fr wal ->
+  repr_val_LambdaANF_Codegen fenv nenv host_function (M.set x v rho) val sr fr wal.
+Proof.
+  intros. inv H0.
+  { (* constr *)
+    have indPrinciple := repr_val_constr_args_LambdaANF_Codegen_mut fenv nenv host_function
+    (fun (rho : LambdaANF.eval.env) (v : cps.val) (s : datatypes.store_record host_function)
+     (f : frame) (w : wasm_value) (H: repr_val_LambdaANF_Codegen fenv nenv host_function rho v s f w) =>
+         (forall x val,
+            rho ! x = None ->
+            repr_val_LambdaANF_Codegen fenv nenv host_function (M.set x val rho) v s f w)
+    )
+    (fun (rho : LambdaANF.eval.env) (l : seq cps.val) (s : datatypes.store_record host_function) (f : frame) (i : immediate)
+         (H: repr_val_constr_args_LambdaANF_Codegen fenv nenv host_function rho l s f i) =>
+         (forall x val,
+            rho ! x = None ->
+            repr_val_constr_args_LambdaANF_Codegen fenv nenv host_function (M.set x val rho) l s f i)
+    ).
+   eapply indPrinciple in H7; clear indPrinciple; intros.
+   { econstructor; eauto. }
+   { econstructor; eauto. }
+   { econstructor; eauto. rewrite M.gso. eassumption. congruence. }
+   { constructor. }
+   { econstructor; eauto. }
+   { assumption. } }
+  { (* fn*)
+  assert ((M.set x v rho) ! x0 = Some (Vfun rho' fds f)). {
+    rewrite M.gso; auto. congruence. } econstructor; eauto. }
+Qed.
+
+Lemma val_relation_depends_on_mem_smaller_than_gmp_and_funcs : forall rho v sr sr' m m' fr fr' gmp gmp' value,
     f_inst fr = f_inst fr' ->
     sr.(s_funcs) = sr'.(s_funcs) ->
     nth_error sr.(s_mems)  0 = Some m ->
@@ -1274,14 +1312,14 @@ Lemma val_relation_depends_on_mem_smaller_than_gmp_and_funcs : forall v sr sr' m
     gmp' >= gmp ->
     (forall a, (a + 4 <= N.of_nat gmp)%N -> load_i32 m a = load_i32 m' a) ->
 
-    repr_val_LambdaANF_Codegen fenv nenv host_function v sr fr value ->
-    repr_val_LambdaANF_Codegen fenv nenv host_function v sr' fr' value.
+    repr_val_LambdaANF_Codegen fenv nenv host_function rho v sr fr value ->
+    repr_val_LambdaANF_Codegen fenv nenv host_function rho v sr' fr' value.
 Proof.
   intros. inv H9.
   (* constructor value *)
   { have indPrinciple := repr_val_constr_args_LambdaANF_Codegen_mut fenv nenv host_function
-    (fun (v : cps.val) (s : datatypes.store_record host_function) (f : frame) (w : wasm_value)
-                       (H: repr_val_LambdaANF_Codegen fenv nenv host_function v s f w) =>
+    (fun (rho : LambdaANF.eval.env) (v : cps.val) (s : datatypes.store_record host_function)
+     (f : frame) (w : wasm_value) (H: repr_val_LambdaANF_Codegen fenv nenv host_function rho v s f w) =>
          (forall a s' f' m m',
                 f_inst f = f_inst f' ->
                 s_funcs s = s_funcs s' ->
@@ -1294,10 +1332,10 @@ Proof.
                 (Z.of_nat gmp' + 4 <= Z.of_N (mem_length m') < Wasm_int.Int32.modulus)%Z ->
                 gmp' >= gmp ->
                 (forall a, (a + 4<= N.of_nat gmp)%N -> load_i32 m a = load_i32 m' a) ->
-                    repr_val_LambdaANF_Codegen fenv nenv host_function v s' f' w)
+                    repr_val_LambdaANF_Codegen fenv nenv host_function rho v s' f' w)
     )
-    (fun (l : seq cps.val) (s : datatypes.store_record host_function) (f : frame) (i : immediate)
-                       (H: repr_val_constr_args_LambdaANF_Codegen fenv nenv host_function l s f i) =>
+    (fun (rho : LambdaANF.eval.env) (l : seq cps.val) (s : datatypes.store_record host_function) (f : frame) (i : immediate)
+                       (H: repr_val_constr_args_LambdaANF_Codegen fenv nenv host_function rho l s f i) =>
          (forall a s' f' m m',
                 f_inst f = f_inst f' ->
                 s_funcs s = s_funcs s' ->
@@ -1310,7 +1348,7 @@ Proof.
                 (Z.of_nat gmp' + 4 <= Z.of_N (mem_length m') < Wasm_int.Int32.modulus)%Z ->
                 gmp' >= gmp ->
                 (forall a, (a + 4 <= N.of_nat gmp)%N -> load_i32 m a = load_i32 m' a) ->
-                   repr_val_constr_args_LambdaANF_Codegen fenv nenv host_function l s' f' i)
+                   repr_val_constr_args_LambdaANF_Codegen fenv nenv host_function rho l s' f' i)
     ). eapply indPrinciple in H16; intros; clear indPrinciple; try eassumption; try lia.
     { assert (gmp = gmp0). { assert (Ht: nat_to_i32 gmp = nat_to_i32 gmp0) by congruence.
                              inv Ht. rewrite Wasm_int.Int32.Z_mod_modulus_id in H14; try lia.
@@ -1326,7 +1364,7 @@ Proof.
       assert (m = m0) by congruence. subst m0.
       assert (m1 = m2) by congruence. subst m2. subst.
       econstructor; eauto. lia. rewrite <- H25; auto; try lia. }
-    { econstructor; eauto. erewrite <- e1. congruence. }
+    { econstructor; eauto. erewrite <- e2. congruence. }
     { econstructor. }
     { assert (gmp = gmp0). {
          assert (Ht: nat_to_i32 gmp = nat_to_i32 gmp0) by congruence.
@@ -1349,12 +1387,12 @@ Proof.
   { econstructor; eauto. rewrite <- H0. eassumption. }
 Qed.
 
-Lemma result_val_LambdaANF_Codegen_depends_on_finst : forall val s f f',
+Lemma result_val_LambdaANF_Codegen_depends_on_finst : forall rho val s f f',
   f_inst f = f_inst f' ->
-  result_val_LambdaANF_Codegen val s f ->
-  result_val_LambdaANF_Codegen val s f'.
+  result_val_LambdaANF_Codegen rho val s f ->
+  result_val_LambdaANF_Codegen rho val s f'.
 Proof.
-  intros ? ? ? ? Hfinst Hres.
+  intros ? ? ? ? ? Hfinst Hres.
   unfold result_val_LambdaANF_Codegen in *.
   destruct Hres as [[res [wal [H1 [H2 H3]]]] | Hres].
   { left. exists res, wal. repeat (split; try congruence).
@@ -2130,12 +2168,12 @@ Proof.
         cbn in *; lia.
 Qed.
 
-Lemma value_bounds : forall wal v sr fr,
+Lemma value_bounds : forall rho wal v sr fr,
   INV_num_functions_upper_bound sr ->
-  repr_val_LambdaANF_Codegen fenv nenv host_function v sr fr wal ->
+  repr_val_LambdaANF_Codegen fenv nenv host_function rho v sr fr wal ->
  (-1 < Z.of_nat (wasm_value_to_immediate wal) < Wasm_int.Int32.modulus)%Z.
 Proof.
-  intros ? ? ? ? Hinv H.
+  intros ? ? ? ? ? Hinv H.
   inv H.
   - (* constr. value *) cbn. lia.
   - (* function value *) cbn.
@@ -2143,17 +2181,17 @@ Proof.
     unfold INV_num_functions_upper_bound in Hinv. lia.
 Qed.
 
-Lemma extract_constr_arg : forall n vs v sr fr addr m,
+Lemma extract_constr_arg : forall rho n vs v sr fr addr m,
   INV_num_functions_upper_bound sr ->
   nthN vs n = Some v ->
   nth_error (s_mems sr) 0 = Some m ->
   (* addr points to the first arg after the constructor tag *)
-  repr_val_constr_args_LambdaANF_Codegen fenv nenv host_function vs sr fr addr ->
+  repr_val_constr_args_LambdaANF_Codegen fenv nenv host_function rho vs sr fr addr ->
   exists bs wal, load m (N.of_nat addr + 4 * n) 0%N 4 = Some bs /\
              VAL_int32 (wasm_value_to_i32 wal) = wasm_deserialise bs T_i32 /\
-             repr_val_LambdaANF_Codegen fenv nenv host_function v sr fr wal.
+             repr_val_LambdaANF_Codegen fenv nenv host_function rho v sr fr wal.
 Proof.
-  intros n vs v sr fr addr m Hinv H H1 H2. generalize dependent v. generalize dependent n. generalize dependent m.
+  intros rho n vs v sr fr addr m Hinv H H1 H2. generalize dependent v. generalize dependent n. generalize dependent m.
   induction H2; intros. 1: inv H.
   assert (n = N.of_nat (N.to_nat n)) by lia. rewrite H8 in H7. generalize dependent v0.
   induction (N.to_nat n); intros.
@@ -2161,7 +2199,7 @@ Proof.
     inv H7. assert (m = m0) by congruence. subst m0. rewrite N.add_comm.
     unfold load_i32 in H3. destruct (load m (N.of_nat addr) 0%N 4) eqn:Hl; inv H3.
     exists b. exists wal. repeat split. rewrite <- Hl. reflexivity. unfold wasm_value_to_i32.
-    have H'' := value_bounds wal.
+    have H'' := value_bounds rho wal.
     unfold wasm_deserialise. f_equal. f_equal.
     have H' := decode_int_bounds _ _ _ Hl.
     rewrite Wasm_int.Int32.Z_mod_modulus_id in H8; try lia.
@@ -2464,8 +2502,8 @@ Lemma memory_grow_reduce_need_grow_mem {lenv} : forall grow state s f gmp m,
            sglob_val (host_function:=host_function) s' (f_inst f) global_mem_ptr = Some (VAL_int32 (nat_to_i32 v_gmp)) ->
            (Z.of_nat v_gmp < Wasm_int.Int32.modulus)%Z ->
            (Z.of_nat v_gmp + Z.of_N page_size < Z.of_N (mem_length m))%Z) /\
-        (forall wal val, repr_val_LambdaANF_Codegen fenv nenv host_function val s f wal ->
-                         repr_val_LambdaANF_Codegen fenv nenv host_function val s' f wal))
+        (forall rho wal val, repr_val_LambdaANF_Codegen fenv nenv host_function rho val s f wal ->
+                         repr_val_LambdaANF_Codegen fenv nenv host_function rho val s' f wal))
       \/ (sglob_val (host_function:=host_function) s' (f_inst f) result_out_of_mem = Some (VAL_int32 (nat_to_i32 1)))).
 Proof with eauto.
   (* grow memory if necessary *)
@@ -2621,8 +2659,8 @@ Lemma memory_grow_reduce_already_enough_mem {lenv} : forall grow state s f gmp m
            sglob_val (host_function:=host_function) s' (f_inst f) global_mem_ptr = Some (VAL_int32 (nat_to_i32 v_gmp)) ->
            (Z.of_nat v_gmp < Wasm_int.Int32.modulus)%Z ->
            (Z.of_nat v_gmp + Z.of_N page_size < Z.of_N (mem_length m))%Z) /\
-        (forall wal val, repr_val_LambdaANF_Codegen fenv nenv host_function val s f wal ->
-                         repr_val_LambdaANF_Codegen fenv nenv host_function val s' f wal))
+        (forall rho wal val, repr_val_LambdaANF_Codegen fenv nenv host_function rho val s f wal ->
+                         repr_val_LambdaANF_Codegen fenv nenv host_function rho val s' f wal))
       \/ (sglob_val (host_function:=host_function) s' (f_inst f) result_out_of_mem = Some (VAL_int32 (nat_to_i32 1)))).
 Proof with eauto.
   destruct exists_i32 as [my_i32 _].
@@ -2736,8 +2774,8 @@ Lemma memory_grow_reduce {lenv} : forall grow state s f,
            sglob_val (host_function:=host_function) s' (f_inst f) global_mem_ptr = Some (VAL_int32 (nat_to_i32 v_gmp)) ->
            (Z.of_nat v_gmp < Wasm_int.Int32.modulus)%Z ->
            (Z.of_nat v_gmp + Z.of_N page_size < Z.of_N (mem_length m))%Z) /\
-        (forall wal val, repr_val_LambdaANF_Codegen fenv nenv host_function val s f wal ->
-                         repr_val_LambdaANF_Codegen fenv nenv host_function val s' f wal))
+        (forall rho wal val, repr_val_LambdaANF_Codegen fenv nenv host_function rho val s f wal ->
+                         repr_val_LambdaANF_Codegen fenv nenv host_function rho val s' f wal))
       \/ (sglob_val (host_function:=host_function) s' (f_inst f) result_out_of_mem = Some (VAL_int32 (nat_to_i32 1)))).
 Proof with eauto.
   (* grow memory if necessary *)
@@ -3058,7 +3096,7 @@ Lemma store_constr_args_reduce {lenv} : forall ys offset vs sargs state rho s f 
   (* memory relation: ys are available as locals in frame f *)
   (forall y, In y ys -> (exists v6 val, M.get y rho = Some v6
                                      /\ stored_in_locals (lenv:=lenv) nenv y val f
-                                     /\ repr_val_LambdaANF_Codegen fenv nenv _ v6 s f val)) ->
+                                     /\ repr_val_LambdaANF_Codegen fenv nenv _ rho v6 s f val)) ->
   exists s', reduce_trans
                   (state, s, f, [seq AI_basic i | i <- sargs])
                   (state, s', f, [])
@@ -3067,7 +3105,7 @@ Lemma store_constr_args_reduce {lenv} : forall ys offset vs sargs state rho s f 
             /\ sglob_val (host_function:=host_function) s' (f_inst f)
                  constr_alloc_ptr = Some (VAL_int32 (nat_to_i32 v_cap))
             /\ (0 <= Z.of_nat v_cap < Wasm_int.Int32.modulus)%Z
-            /\ repr_val_constr_args_LambdaANF_Codegen fenv nenv _ vs s' f (4 + (4*offset) + v_cap)
+            /\ repr_val_constr_args_LambdaANF_Codegen fenv nenv _ rho vs s' f (4 + (4*offset) + v_cap)
             /\ sglob_val (host_function:=host_function) s' (f_inst f)
                  global_mem_ptr = Some (VAL_int32 (nat_to_i32 ((4 + (4*offset) + v_cap) + 4 * (length ys))))
             /\ s_funcs s = s_funcs s'
@@ -3199,7 +3237,7 @@ Proof.
       exists (v6 : cps.val) (val : wasm_value),
         rho ! y = Some v6 /\
         stored_in_locals (lenv:=lenv) nenv y val f /\
-        repr_val_LambdaANF_Codegen fenv nenv host_function v6 s_before_IH f val)). {
+        repr_val_LambdaANF_Codegen fenv nenv host_function rho v6 s_before_IH f val)). {
         intros. assert (Htmp : In y0 (y :: ys)) by (right; assumption).
         destruct (HmemR _ Htmp) as [val' [wal' [? [? ?]]]].
         subst s'. exists val', wal'. repeat split; try assumption.
@@ -3341,7 +3379,7 @@ Lemma store_constr_reduce {lenv} : forall state s f rho ys (vs : list cps.val) t
          exists (v6 : cps.val) (val : wasm_value),
            rho ! y = Some v6 /\
            stored_in_locals (lenv:=lenv) nenv y val f /\
-           repr_val_LambdaANF_Codegen fenv nenv host_function v6 s f val) ->
+           repr_val_LambdaANF_Codegen fenv nenv host_function rho v6 s f val) ->
   (Z.of_nat (length ys) <= max_constr_args)%Z ->
   Forall_statements_in_seq (set_nth_constr_arg (lenv:=lenv) fenv nenv) ys sargs ->
   get_list ys rho = Some vs ->
@@ -3362,7 +3400,8 @@ Lemma store_constr_reduce {lenv} : forall state s f rho ys (vs : list cps.val) t
       (* cap points to value *)
       /\ (exists cap_v wasmval, sglob_val s' (f_inst f) constr_alloc_ptr = Some (VAL_int32 cap_v)
           /\ wasm_value_to_i32 wasmval = cap_v
-          /\ repr_val_LambdaANF_Codegen fenv nenv  _ (Vconstr t vs) s' f wasmval).
+          /\ repr_val_LambdaANF_Codegen fenv nenv  _ rho (Vconstr t vs) s' f wasmval). (* TODO:
+          vlt. muss das rho hier das neue nach der Zuweisung sein? *)
 Proof.
   intros ? ? ? ? ? ? ? ? Hinv HenoughM HmemR Hmaxargs Hsetargs Hrho.
 
@@ -3456,7 +3495,7 @@ In y ys ->
 exists (v6 : cps.val) (val : wasm_value),
   rho ! y = Some v6 /\
   stored_in_locals (lenv:=lenv) nenv y val f /\
-  repr_val_LambdaANF_Codegen fenv nenv host_function v6 s_before_args f val). {
+  repr_val_LambdaANF_Codegen fenv nenv host_function rho v6 s_before_args f val). {
     intros y Hy. apply HmemR in Hy. destruct Hy as [val [wal [Hrho' [Hylocal Hval]]]].
     exists val, wal. repeat (split; auto).
 
@@ -3530,13 +3569,13 @@ exists (v6 : cps.val) (val : wasm_value),
 Qed.
 
 
-Inductive const_val_list : list cps.val -> store_record -> frame -> list nat -> Prop :=
-  | CV_nil  : forall s f, const_val_list [] s f []
-  | CV_cons : forall s f v vs n w ns,
-       repr_val_LambdaANF_Codegen fenv nenv _ v s f w ->
+Inductive const_val_list : LambdaANF.eval.env -> list cps.val -> store_record -> frame -> list nat -> Prop :=
+  | CV_nil  : forall rho s f, const_val_list rho [] s f []
+  | CV_cons : forall rho s f v vs n w ns,
+       repr_val_LambdaANF_Codegen fenv nenv _ rho v s f w ->
        n = wasm_value_to_immediate w ->
-       const_val_list vs s f ns ->
-       const_val_list (v::vs) s f (n::ns).
+       const_val_list rho vs s f ns ->
+       const_val_list rho (v::vs) s f (n::ns).
 
 
 Lemma map_const_const_list : forall args,
@@ -3554,7 +3593,7 @@ Lemma fun_args_reduce {lenv} : forall state fr sr fds (ys : seq cps.var) rho vs 
   exists args,
     reduce_trans (state, sr, fr, map AI_basic args_instr)
                  (state, sr, fr, (map (fun a => AI_basic (BI_const (nat_to_value a))) args))
-    /\ const_val_list vs sr fr args.
+    /\ const_val_list rho vs sr fr args.
 Proof.
   intros ? ? ? ? ? ? ? ? ? ? Hinv Hgetlist HrelM Hargs.
   generalize dependent f. generalize dependent rho. generalize dependent sr.
@@ -3699,7 +3738,11 @@ Theorem repr_bs_LambdaANF_Codegen_related :
       (* protected_id_not_bound_id rho e ->
       unique_bindings_env rho e -> *)
       (* functions_not_bound p rho e -> (* function names in p/rho not bound in e *) *)
-      forall (hs : host_state) (sr : store_record) (f : frame) (fds : fundefs) (instructions : list basic_instruction) (*(k : cont) (max_alloc : Z) (fu : function) *),
+      forall (hs : host_state) (sr : store_record) (f : frame) (fds : fundefs)
+             (instructions : list basic_instruction),
+
+        (* fds only on toplevel*)
+        (forall x rho' fds' f', rho ! x = Some (Vfun rho' fds' f') -> fds' = fds) ->
 
         (* invariants *)
         INV lenv sr f ->
@@ -3709,13 +3752,13 @@ Theorem repr_bs_LambdaANF_Codegen_related :
 
         (* relates a LambdaANF evaluation environment [rho] to a WASM environment [store/frame] (free variables in e) *)
         rel_mem_LambdaANF_Codegen (lenv:=lenv) fenv nenv _ e rho sr f fds ->
-        exists (sr' : store_record) (f' : frame),
+        exists rho_res (sr' : store_record) (f' : frame),
           reduce_trans (hs, sr, f, map AI_basic instructions) (hs, sr', f', []) /\
           (* value sr'.res points to value related to v *)
-          result_val_LambdaANF_Codegen v sr' f' /\ f_inst f = f_inst f'.
+          result_val_LambdaANF_Codegen rho_res v sr' f' /\ f_inst f = f_inst f'.
 Proof with eauto.
   intros lenv HenvsDisjoint HlenvInjective rho v e n HeRestr Hev. generalize dependent lenv.
-  induction Hev; intros lenv HenvsDisjoint HlenvInjective state sr fr fds instructions Hinv Hrepr_e Hrel_m.
+  induction Hev; intros lenv HenvsDisjoint HlenvInjective state sr fr fds instructions Hfds Hinv Hrepr_e Hrel_m.
   - (* Econstr *)
     assert (Hmaxargs: (Z.of_nat (Datatypes.length ys) <= max_constr_args)%Z). { now inv HeRestr. }
 
@@ -3742,7 +3785,7 @@ Proof with eauto.
            exists (v6 : cps.val) (val : wasm_value),
              rho ! y = Some v6 /\
              stored_in_locals (lenv:=lenv) nenv y val fr /\
-             repr_val_LambdaANF_Codegen fenv nenv host_function v6 s' fr val)). {
+             repr_val_LambdaANF_Codegen fenv nenv host_function rho v6 s' fr val)). {
               destruct Hrel_m as [_ Hvar]. intros.
         assert (Hocc: occurs_free (Econstr x t ys e) y) by (constructor; auto).
         apply Hvar in Hocc. destruct Hocc as [val [wal [Hrho [Hloc Hval]]]].
@@ -3761,6 +3804,17 @@ Proof with eauto.
 
       remember ({|f_locs := set_nth (VAL_int32 (wasm_value_to_i32 wal)) (f_locs fr) x' (VAL_int32 (wasm_value_to_i32 wal));
       f_inst := f_inst fr|}) as f_before_IH.
+
+      assert (Hfds_before_IH: (forall (x : positive) (rho'0 : M.t cps.val)
+        (fds' : fundefs) (f' : var), rho' ! x = Some (Vfun rho'0 fds' f') -> fds' = fds)). {
+        intros x1 rho'0 fds' f' Hfds'.
+        subst rho'.
+        destruct (var_dec x x1).
+        (* x=x1 *)
+        { subst x1. rewrite M.gss in Hfds'. inv Hfds'. }
+        (* x<>x1 *)
+        { rewrite M.gso in Hfds'; auto. now apply Hfds in Hfds'. }
+      }
 
       assert (Hinv_before_IH: INV lenv s_v f_before_IH). {
         eapply update_local_preserves_INV; try eassumption.
@@ -3791,10 +3845,10 @@ Proof with eauto.
 
       assert (HeRestr' : expression_restricted e). { now inv HeRestr. }
 
-      have IH := IHHev HeRestr' _ HenvsDisjoint HlenvInjective state _ _ _ _ Hinv_before_IH Hexp Hrel_m_v.
-      destruct IH as [s_final [f_final [Hred_IH [Hval Hfinst]]]]. cbn in Hfinst.
+      have IH := IHHev HeRestr' _ HenvsDisjoint HlenvInjective state _ _ _ _ Hfds_before_IH Hinv_before_IH Hexp Hrel_m_v.
+      destruct IH as [rho_final [s_final [f_final [Hred_IH [Hval Hfinst]]]]]. cbn in Hfinst.
 
-      exists s_final. exists f_final. split.
+      exists rho_final, s_final, f_final. split.
       (* steps *)
       eapply rt_trans. apply app_trans. apply Hred. cbn.
 
@@ -3841,7 +3895,7 @@ Proof with eauto.
     apply /ssrnat.leP. apply nth_error_Some. congruence. subst. reflexivity. apply rt_refl. cbn.
     apply Hred_IH. split. assumption. subst f_before_IH. cbn in Hfinst. congruence. }}
     { (* grow mem failed *)
-    eexists. eexists. split. eapply rt_trans. apply app_trans. apply Hred.
+    eexists. eexists. eexists. split. eapply rt_trans. apply app_trans. apply Hred.
     dostep. elimr_nary_instr 0. apply r_get_global. eassumption.
     dostep. elimr_nary_instr 2. constructor. apply rs_relop.
     dostep'. constructor. apply rs_if_true. intro Hcontra. inv Hcontra.
@@ -3863,7 +3917,7 @@ Proof with eauto.
       inv Hlocal. destruct H.
 
       have I := Hinv. destruct I as [_ [_ [_ [_ [_ [_ [_ [_ [_ [HfnsUpperBound [_ [_ [HlocalBound _]]]]]]]]]]]]].
-      have Hextr := extract_constr_arg n vs v _ _ _ _ HfnsUpperBound H0 H5 H12.
+      have Hextr := extract_constr_arg rho n vs v _ _ _ _ HfnsUpperBound H0 H5 H13.
       destruct Hextr as [bs [wal [Hload [Heq Hbsval]]]].
 
       assert (Hrm: rel_mem_LambdaANF_Codegen (lenv:=lenv) fenv nenv host_function e (map_util.M.set x v rho) sr
@@ -3878,11 +3932,12 @@ Proof with eauto.
           econstructor; try eassumption; eauto. *) admit. (* x not a fundef *)
 
           (* x <> x1*) rewrite M.gso in H6; auto.
-                       have H' := Hfun _ _ _ _  errMsg H6 H9.
+                       have H' := Hfun _ _ _ _  errMsg H6 H8.
                        destruct H' as [i [Htf [Hval HvalClosed]]].
                        exists i. split; auto. split; auto.
-                       eapply val_relation_depends_on_finst; try eassumption.
-                       reflexivity. }
+                       apply val_relation_rho_depends_on_bound_vars.
+                       (* x not bound yet *) admit.
+                       eapply val_relation_depends_on_finst; try eassumption. reflexivity. }
 
         destruct (var_dec x x1).
         { (* x = x1 *)
@@ -3891,12 +3946,13 @@ Proof with eauto.
           rewrite map_util.M.gsspec.
           apply peq_true.
           split; auto. exists x'. split. inv Hx'. intro.
-          unfold translate_var in H9. unfold translate_var.
-          destruct (lenv ! x); auto. inv H9. cbn.
+          unfold translate_var in H8. unfold translate_var.
+          destruct (lenv ! x); auto. inv H8. cbn.
           unfold wasm_deserialise in Heq. rewrite -Heq.
           have Hl := HlocalBound _ _ Hx'. apply nth_error_Some in Hl.
           apply notNone_Some in Hl. destruct Hl.
           eapply set_nth_nth_error_same. eassumption.
+          eapply val_relation_rho_depends_on_bound_vars. admit. (* x not bound yet *)
           eapply val_relation_depends_on_finst; try eassumption; auto. }
 
         { (* x <> x1 *)
@@ -3911,15 +3967,27 @@ Proof with eauto.
           assert (x1' <> x'). { intro. subst x1'.
             inv Hx'. unfold translate_var in H11.
             destruct (lenv ! x) eqn:Heqn. 2: inv H11.
-            specialize H9 with ""%bs. unfold translate_var in H9. inv H11.
-            destruct (lenv ! x1) eqn:Heqn'; inv H9.
+            specialize H8 with ""%bs. unfold translate_var in H8. inv H11.
+            destruct (lenv ! x1) eqn:Heqn'; inv H8.
             have Hcontra := HlenvInjective _ _ _ _ n0 Heqn Heqn'.
             now apply Hcontra. }
 
           exists x1'. split; auto.
           rewrite set_nth_nth_error_other; auto. eapply HlocalBound. eassumption.
+          eapply val_relation_rho_depends_on_bound_vars. (* x not bound yet *) admit.
           eapply val_relation_depends_on_finst; try eassumption; auto. }
      }
+
+     assert (Hfds': (forall (x1 : positive) (rho' : M.t cps.val)
+            (fds' : fundefs) (f' : var),
+      (map_util.M.set x v rho) ! x1 = Some (Vfun rho' fds' f') -> fds' = fds)). {
+        intros x1 rho' fds' f' Hfds'.
+        destruct (var_dec x x1).
+        (* x=x1 *)
+        { subst x1. rewrite M.gss in Hfds'. inv Hfds'. inv Hbsval. now apply Hfds in H11. }
+        (* x<>x1 *)
+        { rewrite M.gso in Hfds'; auto. now apply Hfds in Hfds'. }
+      }
 
      assert (Hinv': INV lenv sr {| f_locs := set_nth (wasm_deserialise bs T_i32)
                                 (f_locs fr) x' (wasm_deserialise bs T_i32);
@@ -3930,9 +3998,9 @@ Proof with eauto.
 
     assert (HeRestr' : expression_restricted e). { now inv HeRestr. }
 
-     have IH := IHHev HeRestr' _ HenvsDisjoint HlenvInjective state sr _ _ e' Hinv' H7 Hrm. destruct IH as [sr' [f' [Hred [Hval Hfinst]]]]. cbn in Hfinst.
+     have IH := IHHev HeRestr' _ HenvsDisjoint HlenvInjective state sr _ _ e' Hfds' Hinv' H7 Hrm. destruct IH as [rho' [sr' [f' [Hred [Hval Hfinst]]]]]. cbn in Hfinst.
 
-      exists sr'. exists f'. cbn. split.
+      eexists rho', sr', f'. cbn. split.
       { (* take steps *)
       have Htmp := Hy'. inv Htmp.
 
@@ -3968,7 +4036,6 @@ Proof with eauto.
       rewrite Har. apply Hload.
 
       (* save result in x' *)
-      have Hx := H8. inv H8. cbn.
       (* dostep' with fr *)
       eapply rt_trans with (y := (?[hs], ?[sr], {|
              f_locs :=
@@ -3980,8 +4047,7 @@ Proof with eauto.
       apply r_set_local with (vd := (wasm_deserialise bs T_i32)). reflexivity.
       apply /ssrnat.leP. apply HlocalBound in Hx'. assumption.
       reflexivity. cbn. apply Hred.
-      }
-      split. apply Hval. assumption.
+      } auto.
     }
   - (* Ecase *)
     { generalize dependent y. generalize dependent instructions. induction cl; intros; subst. inv H1. destruct a. rename c0 into t0.
@@ -4008,15 +4074,14 @@ Proof with eauto.
 
       assert (HeRestr': expression_restricted e). { inv HeRestr. now inv H1. }
 
-      have IH := IHHev HeRestr' _ HenvsDisjoint HlenvInjective state _ _ _ _ Hinv H9 Hrel. destruct IH as [sr' [fr' [Hstep Hval]]].
+      have IH := IHHev HeRestr' _ HenvsDisjoint HlenvInjective state _ _ _ _ Hfds Hinv H9 Hrel. destruct IH as [rho' [sr' [fr' [Hstep Hval]]]].
 
-    exists sr'. exists fr'.
-    split. {
-    (* steps *)
+    exists rho', sr', fr'. split.
+    { (* steps *)
     dostep. elimr_nary_instr 0.
     apply r_get_local. eassumption.
 
-    unfold load_i32 in H10.
+    unfold load_i32 in H11.
     destruct (load m (N.of_nat addr) (N.of_nat 0) 4) eqn:Hload.
 
     dostep. elimr_nary_instr 1. eapply r_load_success. apply Hlinmem. eassumption.
@@ -4030,12 +4095,12 @@ Proof with eauto.
     dostep'. constructor. apply rs_if_true.
     cbn. unfold nat_to_i32. unfold tag_to_i32.
     unfold Wasm_int.Int32.eq.
-    cbn in Hload. rewrite Hload in H10. subst. injection H10 => H10'.
+    cbn in Hload. rewrite Hload in H11. subst. injection H11 => H11'.
     destruct (zeq (Wasm_int.Int32.unsigned (Wasm_int.Int32.repr (decode_int b)))
       (Wasm_int.Int32.unsigned (Wasm_int.Int32.repr (Z.of_nat (Pos.to_nat t))))) eqn:Heq. discriminate. contradiction.
 
     dostep'. constructor. eapply rs_block with (vs := []); auto. unfold to_e_list. cbn.
-    eapply reduce_trans_label. apply Hstep. unfold load_i32 in H10. rewrite Hload in H10. inv H10. }
+    eapply reduce_trans_label. apply Hstep. unfold load_i32 in H11. rewrite Hload in H11. inv H11. }
     assumption. }
 
     (* t0 <> t *)
@@ -4047,7 +4112,7 @@ Proof with eauto.
     assert (HeRestr' : expression_restricted (Ecase y cl)). { inv HeRestr. inv H3.
                                                                now constructor. }
     have IH := IHcl H10 H1 _ _ HeRestr' H H12 Hrel.
-    destruct IH as [sr' [f' [Hred [Hval Hfinst]]]].
+    destruct IH as [rho' [sr' [f' [Hred [Hval Hfinst]]]]].
 
     (* t <> t0 *)
     assert (Hy : occurs_free (Ecase y ((t0, e0) :: cl)) y) by constructor.
@@ -4064,27 +4129,27 @@ Proof with eauto.
     inv Hlocal. destruct H3.
     rewrite H3 in H0. inv H0. rewrite H4 in H. inv H.
 
-    eexists. eexists. cbn. split.
+    eexists. eexists. eexists. cbn. split.
 
     (* execute instructions *)
     dostep. elimr_nary_instr 0.
     apply r_get_local. eassumption.
 
      assert (Harith: (N.of_nat addr) = (Wasm_int.N_of_uint i32m (wasm_value_to_i32 (Val_ptr addr)))). cbn. rewrite Wasm_int.Int32.Z_mod_modulus_id; lia. cbn.
-    rewrite Harith in H17.
+    rewrite Harith in H18.
      unfold load_i32 in H8.
     destruct (load m (Wasm_int.N_of_uint i32m (wasm_value_to_i32 (Val_ptr addr)))
          (N.of_nat 0) 4) eqn:Hload.
      { dostep. elimr_nary_instr 1.
        eapply r_load_success.
        apply Hlinmem. eassumption.
-       apply Hload. unfold load_i32 in H17. rewrite Hload in H17.
+       apply Hload. unfold load_i32 in H18. rewrite Hload in H18.
        assert (wasm_deserialise b T_i32 = VAL_int32 (tag_to_i32 t)). {
        inv H15. unfold wasm_deserialise. f_equal. unfold tag_to_i32. cbn.
        cbn in Hload.
        rewrite Wasm_int.Int32.Z_mod_modulus_id in Hload; try lia.
        replace (Z.to_N (Z.of_nat addr)) with (N.of_nat addr) in Hload by lia.
-       apply decode_int_bounds in Hload. inv H17.
+       apply decode_int_bounds in Hload. inv H18.
        rewrite Wasm_int.Int32.Z_mod_modulus_id in H15; auto. rewrite H15.
        rewrite Wasm_int.Int32.Z_mod_modulus_id; auto.
 
@@ -4110,7 +4175,7 @@ Proof with eauto.
 
       dostep'. constructor. eapply rs_block with (vs := []); eauto. cbn.
       eapply reduce_trans_label. unfold to_e_list. apply Hred.
-     } unfold load_i32 in H17. rewrite Hload in H17. inv H17. split; assumption. }
+     } unfold load_i32 in H18. rewrite Hload in H18. inv H18. split; eassumption. }
   - (* Eapp *)
     inv Hrepr_e. rename args' into args_instr. inv H8.
     { (* indirect call*)
@@ -4126,6 +4191,11 @@ Proof with eauto.
                   (map nat_to_value args ++
                      (repeat (nat_to_value 0) (length (collect_local_variables e))))
                   (f_inst fr)) as f_before_IH.
+
+       assert (Hfds_before_IH: (forall (x : positive) (rho' : M.t cps.val)
+        (fds' : fundefs) (f' : var),
+      rho'' ! x = Some (Vfun rho' fds' f') -> fds' = fds)). { admit. }
+
        assert (Hinv_before_IH : INV lenv_before_IH sr f_before_IH). {
           subst. eapply init_local_preserves_INV; try eassumption; try reflexivity.
           intros. inv H3. apply local_var_mapping_list in H5. lia. }
@@ -4140,16 +4210,16 @@ Proof with eauto.
       assert (HenvsDisjoint': maps_disjoint fenv lenv_before_IH) by admit. (* true *)
       assert (HlenvInjective': map_injective lenv_before_IH ) by admit. (* true *)
 
-      have IH := IHHev HeRestr' _  HenvsDisjoint' HlenvInjective' state _ _ _ _ Hinv_before_IH Hexpr Hrelm.
-      destruct IH as [sr_final [fr_final [Hred [Hval Hfinst]]]].
+      have IH := IHHev HeRestr' _  HenvsDisjoint' HlenvInjective' state _ _ _ _ Hfds_before_IH Hinv_before_IH Hexpr Hrelm.
+      destruct IH as [rho_final [sr_final [fr_final [Hred [Hval Hfinst]]]]].
       (* execute *)
-      exists sr_final. exists fr_final. split.
+      exists rho_final, sr_final, fr_final. split.
       eapply rt_trans. apply app_trans. apply HfargsRed.
       dostep. apply r_eliml. apply map_const_const_list.
       eapply r_call_indirect_success.
 
       { cbn. unfold stab_addr. unfold stab_index. admit. }
-        admit. admit. admit. subst. cbn in Hfinst. auto. }
+        admit. admit. admit. subst. cbn in Hfinst. split; auto. }
   - (* Eletapp *)   inv Hrepr_e. (* absurd, we require CPS *)
   - (* Efun *)      inv Hrepr_e. (* absurd, fn defs only on topmost level *)
   - (* Eprim_val *) inv Hrepr_e. (* absurd, primitives not supported *)
@@ -4170,9 +4240,9 @@ Proof with eauto.
     specialize INVres with (wasm_value_to_i32 wal).
     destruct INVres as [s' Hs].
 
-    exists s'. eexists fr. cbn.
+    eexists. exists s', fr. cbn. split.
     destruct H2.
-    destruct Hloc as [ilocal [H4 Hilocal]]. split. erewrite H4 in H2. injection H2 => H'. subst. clear H2.
+    destruct Hloc as [ilocal [H4 Hilocal]]. erewrite H4 in H2. injection H2 => H'. subst. clear H2.
     (* execute wasm instructions *)
     dostep. separate_instr. apply r_elimr. eapply r_get_local. eassumption.
     dostep'. apply r_set_global. eassumption.
@@ -4894,14 +4964,14 @@ Qed.
 (* MAIN THEOREM, corresponds to 4.3.1 in Olivier's thesis *)
 Corollary LambdaANF_Codegen_related :
   (* rho is environment containing outer fundefs. e is body of LambdaANF program *)
-  forall (rho : eval.env) (v : cps.val) (e : exp) (n : nat) (vars : list cps.var),
+  forall (v : cps.val) (e : exp) (n : nat) (vars : list cps.var),
   (* restricts the number of args a function can have etc. *)
   expression_restricted e ->
   forall (hs : host_state) module fenv lenv mainidx errMsg,
     forall (sr : store_record) (fr : frame) exports,
 
   (* evaluation of LambdaANF expression *)
-  bstep_e (M.empty _) cenv rho e v n ->
+  bstep_e (M.empty _) cenv (M.empty _) e v n ->
   (* compilation function *)
   LambdaANF_to_WASM nenv cenv e = Ret (module, fenv, lenv) ->
   translate_function_var nenv fenv main_function_var errMsg = Ret mainidx ->
@@ -4915,13 +4985,13 @@ Corollary LambdaANF_Codegen_related :
   (* instiation with the two imported functions *)
   instantiate _ host_instance initial_store module [MED_func (Mk_funcidx 0); MED_func (Mk_funcidx 1)] ((sr, (f_inst fr), exports), None) ->
   (* *)
-  exists (sr' : store_record),
+  exists rho (sr' : store_record),
        reduce_trans (hs, sr,  (Build_frame [] (f_inst fr)), [ AI_basic (BI_call mainidx) ])
                     (hs, sr', (Build_frame [] (f_inst fr)), [])    /\
 
-       result_val_LambdaANF_Codegen fenv nenv _ v sr' fr.
+       result_val_LambdaANF_Codegen fenv nenv _ rho v sr' fr.
 Proof.
-  intros ? ? ? ? ? HeRestr ? ? ? ? ? ? ? ? ? Hstep LANF2WASM Hmainidx Hcenv HvarsEq Hvars Hfreevars Hinst. subst vars.
+  intros ? ? ? ? HeRestr ? ? ? ? ? ? ? ? ? Hstep LANF2WASM Hmainidx Hcenv HvarsEq Hvars Hfreevars Hinst. subst vars.
   remember ({| f_locs := []; f_inst := f_inst fr |}) as f.
   assert (Hmaxfuns : (Z.of_nat match match e with
                                      | Efun _ _ => e
@@ -4961,6 +5031,7 @@ Proof.
   remember (Build_frame (repeat (nat_to_value 0) (length (collect_local_variables e))) (f_inst fr)) as f_before_IH.
   remember (create_local_variable_mapping (collect_local_variables e)) as lenv.
   remember (create_fname_mapping nenv e) as fenv.
+
   assert (Hinv_before_IH: INV fenv nenv _ lenv sr f_before_IH). { subst.
     destruct Hinv as [? [? [? [? [? [? [? [? [? [? [? [? [? ?]]]]]]]]]]]]].
     unfold INV. repeat (split; try assumption).
@@ -5013,7 +5084,7 @@ Proof.
                     _ _ _ _ HeRestr Hstep hs _ _ fds wasm_main_instr Hinv_before_IH.
     TODO: check e vs e0 richtige Variable *)
 
-    exists sr. subst. admit. admit. }
+    eexists. exists sr. subst. admit. admit. }
 
   { (* top exp is not Efun _ _ *)
     rename f0 into fds. assert (fds = Fnil). {
@@ -5026,10 +5097,9 @@ Proof.
     eapply translate_exp_correct in Hexpr; auto.
 
     assert (Hrelm : rel_mem_LambdaANF_Codegen fenv (lenv:=create_local_variable_mapping (collect_local_variables e)) nenv
-            host_function e rho sr f_before_IH Fnil). {
+            host_function e (M.empty _) (* empty hier falsch*) sr f_before_IH Fnil). {
       split.
-      { intros. exfalso. cbn in HsrFuncs.
-        admit. (* absurd, no functions *) }
+      { intros. exfalso. cbn in HsrFuncs. inv H. }
       { intros. exfalso. eauto. }}
 
    assert (HlenvInjective : map_injective (create_local_variable_mapping
@@ -5047,12 +5117,17 @@ Proof.
           (create_local_variable_mapping
              (collect_local_variables e))). admit.
 
+  assert (Hfds_before_IH: (forall (x : positive) (rho' : M.t val)
+           (fds' : fundefs) (f' : var),
+         (M.empty _) ! x = Some (Vfun rho' fds' f') -> fds' = Fnil)). {
+   intros. inv H. }
+
     subst lenv.
     have HMAIN := repr_bs_LambdaANF_Codegen_related cenv funenv fenv nenv finfo_env
-                    rep_env _ host_instance _ HenvsDisjoint HlenvInjective rho _
-                     _ _ HeRestr Hstep hs _ _ _ wasm_main_instr Hinv_before_IH Hexpr Hrelm.
-    destruct HMAIN as [s' [f' [Hred [Hval Hfinst]]]]. cbn.
-    exists s'. split.
+                    rep_env _ host_instance _ HenvsDisjoint HlenvInjective (M.empty _) _
+                     _ _ HeRestr Hstep hs _ _ _ wasm_main_instr Hfds_before_IH Hinv_before_IH Hexpr Hrelm.
+    destruct HMAIN as [rho' [s' [f' [Hred [Hval Hfinst]]]]]. cbn.
+    exists rho', s'. split.
     dostep'. apply r_call. cbn.
     rewrite HinstFuncs. reflexivity.
     dostep'. eapply r_invoke_native with (ves:=[]) (vcs:=[]) (t1s:=[]) (t2s:=[])(f' := f_before_IH); eauto.
@@ -5064,7 +5139,7 @@ Proof.
     eapply reduce_trans_local.
     dostep'. constructor. eapply rs_block with (vs:=[]); eauto. cbn.
     apply reduce_trans_label. apply Hred.
-    eapply result_val_LambdaANF_Codegen_depends_on_finst; try eassumption. subst. cbn in Hfinst. congruence.
+    eapply result_val_LambdaANF_Codegen_depends_on_finst; try eassumption. subst. cbn in Hfinst. congruence. Unshelve. apply (M.empty _).
 Admitted.
 
 (*
